\documentclass{article}

\usepackage{amsmath, amssymb, amsthm}
\newcommand{\reals}{\ensuremath{\mathbb{R}}}
\newcommand{\rats}{\ensuremath{\mathbb{Q}}}
\newcommand{\irats}{\ensuremath{\reals \backslash \rats}}
\newcommand{\nats}{\ensuremath{\mathbb{N}}}
\newcommand{\eps}{\ensuremath{\epsilon}}
\newcommand{\limxy}[2]{\ensuremath{\underset{#1 \to #2 }{\lim}}}
\newcommand{\pt}[1]{\textrm{ #1 }}
\newtheorem{clm}{Claim}

\title{Real Analysis Assignment 11}
\author{Joel Savitz}

\begin{document}

\maketitle

\textbf{Problem 1:}

Define $f_n (x) = \frac{x^2}{2x^2 + (nx -3)^2}$.

If $x = 0$, then $\limxy{n}{\infty} f_n (x) = 0$
since the function is a fraction with numerator $0$.
If $x \neq 0$, then $\limxy{n}{\infty} f_n (x) = 0$
since the expression is a fraction with
a nonzero numerator and a  denominator
with a positive term value that grows arbitrarily
as $n$ increases without bound.
Thus, $\limxy{n}{\infty}f_n(x) = f(x) = 0$.

\begin{clm}
	$f_n(x)$ does not converge uniformly to $f(x)$ on $\reals$.
\end{clm}

\begin{proof}
	We want to show that
	$f_n(x)$ does not converge uniformly to $f(x)$ on $\reals$,
	and we will do so by showing that the negation of the definition
	of uniform convergence is satisfied by $f_n(x)$.
	That is to say,
	$\exists \eps > 0,
	\forall N \in \nats,
	\exists n > N, \exists x \in \reals,
	|f_n(x) - f(x)| \geq \eps$.
	Let $\eps = \frac{1}{2}$
	and $N \in \nats$.
	Then, $\exists n > N$.
	Let $x = \frac{n}{3}$.
	Then, $|f_n(x) - f(x)| = |\frac{(3/n)^2}{2(3/n)^2 + (n(3/n) - 3)^2}| = \frac{1}{2} \geq \eps$,
	so we have that $f_n(x)$
	does not converge uniformly
	to $f(x)$ on $\reals$.
\end{proof}

\textbf{Problem 2:}


Define $f_n (x) = \frac{x^2}{2x^2 + (nx -3)^2}$.

\begin{clm}
	$f_n(x)$ converges uniformly to $f(x)$ on $[\frac{1}{3}, \infty)$.
\end{clm}

\begin{proof}
	We verify the definition of uniform convergence, that
	$\forall \eps > 0,
	\exists N_\eps \in \nats,
	\forall n > N_\eps,
	\forall x \in [\frac{1}{3}, \infty),
	|f_n(x) - f(x)| < \eps$.
	Let $\eps > 0$.
	We examine the consequent to find a suitable value of $N_\eps$.
	Let $n > N_\eps$:
	\begin{align}
		|f_n(x) - f(x)| = & |\frac{x^2}{2x^2 + (nx - 3)^2}| \\
		\pt{(positive num. and denom.)} & = \frac{x^2}{2x^2 + (nx - 3)^2} \\
				< &  \frac{x^2}{(nx - 3)^2} \\
				= & \frac{x^2}{n^2x^2 -6nx + 9} \\
				< & \frac{x^2}{n^2x^2 -6nx}
	\end{align}
	To shrink the denominator further,
	we will replace $6xn$ with a smaller positive term,
	and this will introduce a constraint on $N_\eps$.
	We  use $\frac{1}{2}n^2x^2$:
	\begin{align}
		6nx < & \frac{1}{2}n^2 x^2 \\
		6 < & \frac{1}{2}nx \\
		12 < & nx
	\end{align}
	But since $x \geq \frac{1}{3}$,
	we $12 < \frac{n}{3} \implies 36 < n$.
	We have the constraint $N_\eps \geq 36$.
	Now, we continue with the full examination:
	\begin{align}
		\frac{x^2}{n^2x^2 -6nx} < & \frac{x^2}{n^2x^2 -\frac{1}{2}n^2x^2} \\
					= & \frac{x^2}{\frac{1}{2}n^2x^2} \\
					= & \frac{2}{n^2}
	\end{align}
	If $n > \sqrt{2/\eps}$,
	then $\frac{n^2}{2} > \frac{1}{\eps}$,
	so $\frac{2}{n^2} < \eps$.
	By the archimedian propety,
	we can choose some $N_\eps > \max(36, \sqrt{2/\eps})$,
	and we have
	$\forall \eps > 0,
	\exists N_\eps \in \nats,
	\forall n > N_\eps,
	\forall x \in [\frac{1}{3}, \infty),
	|f_n(x) - f(x)| < \eps$.
	This is exactly the definition that
	$f_n(x)$ converges uniformly to $f(x)$ on $[\frac{1}{3}, \infty)$.
\end{proof}

\textbf{Problem 3:}

Define $f_n(x) = \frac{x^{2n} - 1}{x^{2n} + 1}$.

If $x = 0$, then  $f_n(x) = \frac{0- 1}{0 + 1} = -1$, so $\limxy{n}{\infty} f_n(x) = 0$.

If $0 < |x| < 1$, then by the limit laws,
$\limxy{n}{\infty} f_n(x) = \frac{\limxy{n}{\infty} (x^2)^n - 1}{\limxy{n}{\infty} (x^2)^n + 1}
= \frac{0- 1}{0 + 1} = -1$.

If $|x| = 1$, then $f_n(x) = \frac{1- 1}{1 + 1}  = 0$.

If $|x| > 1$, then $\limxy{n}{\infty}f_n(x)$ looks like it will be $1$.
To show this,
we see that $|f_n(x) - 1| = |\frac{x^{2n} -1}{x^{2n} + 1} - \frac{x^{2n} + 1}{x^{2n} + 1}|
= \frac{2}{x^{2n} + 1} < \frac{2}{x^{2n}}$.
Let $\eps > 0$.
If we set $n > N_\eps > \log_x(\sqrt{2/\eps})$,
then $2n > \log_x(2/\eps)$ and $x^{2n} > \frac{2}{\eps}$,
so $\frac{2}{x^{2n}} < \eps$,
and we have that
$\forall \eps > 0, \exists N_\eps, \forall n > N_\eps, |f_n(x) - 1| < \eps$,
so indeed $|x| > 1 \implies \limxy{n}{\infty} f_n(x) = f(x) = 1$.

We have the following function:
$\limxy{n}{\infty} f_n(x) = f(x) =
\begin{cases}
	-1 & \pt{(if $|x| < 1$)} \\
	 0 & \pt{(if $|x| = 1$)} \\
	 1 & \pt{(if $|x| > 1$)}
\end{cases}$.

\begin{clm}
	$f_n(x)$ converges to $f(x)$ uniformly on $A = [\frac{-1}{3}, \frac{1}{3}]$.
\end{clm}

\begin{proof}
	Since $\forall x \in A, |x| < 1$,
	we have $f(x) = -1$.
	We examine $|f_n(x) - f(x)|$:
	\begin{align}
		|f_n(x) - f(x)| = & |\frac{x^{2n} - 1}{x^{2n} + 1} + 1| \\
		= & |\frac{x^{2n} - 1}{x^{2n} + 1} + \frac{x^{2n} + 1}{x^{2n} + 1}| \\
		= & |\frac{2x^{2n}}{x^{2n} + 1}| \\
		\pt{(positive num. and denom.)} = & \frac{2x^{2n}}{x^{2n} + 1} \\
		\pt{($x^{2n} + 1 > 1$)} < & 2x^{2n}
	\end{align}
	Since $\forall x \in A, |x| \le \frac{1}{3} < \frac{1}{2}$,
	we have $2x^{2n} \le 2 \cdot 3^{-2n} < 2 \cdot 3^{-2n}$,
	and $\limxy{n}{\infty} 2 \cdot 3^{-2n} = 0$.
	% Since $|x| < 1$, we have $\limxy{n}{\infty} 2x^{2n} = 0$.
	Thus $\exists c_n = 2\cdot 3^{-2n}$ where $\forall x \in A, |f_n(x) - f(x)| < c_n$,
	and $\limxy{n}{\infty} c_n = 0$,
	which is true if and only if
	$f_n(x)$ converges to $f(x)$ uniformly on $A = [\frac{-1}{3}, \frac{1}{3}]$.
\end{proof}

\begin{clm}
	$f_n(x)$ does not converge uniformly to $f(x)$ on $A = (0,1)$.
\end{clm}

\begin{proof}
	Consider $|f_n(x) - f(x)|$ on $A$.
	Since $A = (0,1)$, we have $|x| < 1$,
	so $f(x) = -1$.
	Since $x^{2n} < 1$:
	\begin{align}
		|f_n(x) - f(x)| = & |\frac{x^{2n} - 1}{x^{2n} + 1} + 1| \\
		= & |\frac{2x^{2n}}{x^{2n} + 1}| \\
		< & |\frac{2x^{2n}}{x^{2n} + x^{2n}}| \\
		= & |\frac{2x^{2n}}{2x^{2n}}| \\
		= & 1
	\end{align}
	So $1$ is an upper bound of $|f_n(x) - f(x)|$.
	Let $1 > \eps > 0$ and let $x = (1 - \eps)^{1/2n} $.
	Then:
	\begin{align}
		|f_n(x) - f(x)| = & |\frac{x^{2n} - 1}{x^{2n} + 1} + 1| \\
			= & \frac{2x^{2n}}{x^{2n} + 1} \\
			= & \frac{2(1-\eps)}{(1-\eps) + 1} \\
			= & \frac{2-2\eps}{2-\eps} \label{eq666}
	\end{align}
	We verify that (\ref{eq666}) is greater than $1 - \eps$:
	\begin{align}
		\frac{2-2\eps}{2-\eps} > & 1 - \eps \\
		2-2\eps > & (1-\eps)(2-\eps) = 2 - 3\eps + \eps^2 \\
		\eps > & \eps^2
	\end{align}
	This last inequality is true since $0 < \eps < 1$,
	so $1 - \eps$ is not an upper bound of $|f_n(x) - f(x)|$,
	and we have $\underset{x \in A}{\sup}|f_n(x) - f(x)| = 1$.
	Then, $\limxy{n}{\infty}\Big(\underset{x \in A}{\sup}|f_n(x) - f(x)|\Big) = 1 \neq 0$,
	which is true if and only if
	$f_n(x)$ does not converge uniformly to $f(x)$ on $A = (0,1)$.
\end{proof}

\end{document}
